\chapter{Testing}

\begin{equation*}
\frac{e^x}{e^{2x}-e^x}=\frac{e^x}{e^x(e^x-1)}=\frac{1}{e^x-1} - \frac{1}{e^{2x}-e^x}
\end{equation*}

To obtain this expression, we used the fact that:

\begin{equation*}
\frac{1}{e^x(e^x-1)}=\frac{1}{e^x}-\frac{1}{e^{2x}}
\end{equation*}

Now, we can use partial fraction decomposition on the two terms on the right-hand side. For the first term, we have:

\begin{equation*}
\frac{1}{e^x-1}=\frac{A}{e^x-1}
\end{equation*}

Multiplying both sides by $e^x-1$, we get:

\begin{equation*}
1 = A(e^x-1)
\end{equation*}

Solving for $A$, we get $A=1/(e^x-1)$.

For the second term, we have:

\begin{equation*}
\frac{1}{e^{2x}-e^x}=\frac{B}{e^x}-\frac{B}{e^{2x}}
\end{equation*}

Multiplying both sides by $e^{2x}$, we get:

\begin{equation*}
1 = B(e^x - 1)
\end{equation*}

Solving for $B$, we get $B=1/(e^x-1)$.

Therefore, we have:

\begin{equation*}
\frac{e^x}{e^{2x}-e^x}=\frac{1}{e^x-1} - \frac{1}{e^{2x}-e^x}=\frac{1}{e^x-1} - \frac{1}{e^x} + \frac{1}{e^{2x}}
\end{equation*}


